Ping pong protocol (#39)
* Inital simplification refactoring of keys, encryptions, signatures.

* Find keys and add to heap upon receiving message, or decrypting message

* Spike of simulation relation statement

* adding labels to ideal world

* Start Ping Protocol simulation relation.  Wait for now to get IdealWorld update

* issue-less change since it's so fundamental to the real world model

* Simple ping proof stuck

* Remove some cruft

* Some proof automation.  The simulation relation is clearly not right yet.  Not sure this is the right approach

* Successful proof of ping simulation

* Some more automation

* Automated simulation proof.  Working on top level proof.

* WIP.  Need to get a transitivity-like theorem implemented

* Fiddling with some proof automation setup.

* WIP

* Top level proof done.

* Starting to automate proof

* Some proof automation

* neatening up

* Refactoring semantics of simulates.  WIP

* Refactoring WIP

* Finished (needs more automation) proof of ping simulation relation

* Ping protocol proof done again.

* wrote the protocols for auth and enc

* Ping Protocol Correct

* Ping protocol automation

* Remove Makefile.coq.conf which shouldn't be checked in

* set up auth proof with iffy invariant, need invariant for enc proof

* More proof automation in Simulates

* Quick stab at real world enc ping protocol

* Initial step towards simulation relation of simple encrypt/send protocol.  At this point, I need to put in the relevant operational semantics rules, but it looks like this new style of simulation relation (i.e. using a much fewer number of states than all possible interleavings) is going to work.

* Step part of enc ping simulation relation is proven.

* Proof automation for encrypted ping protocol.

* Modularize enc ping (#30)

Simple encryption ping protocols correct

* Simplification of automation

* any thoughts on the hacky boolean return?

* WIP

* making real messages type -> type, added enough message eq for ping

* Timb (#32)

Working labeled ping protocol proof

* Refactor labeled ping protocol to be a universe of unit

* Soundness proof of encrypted ping protocol has been reduced to action_matches proof obligations

* Small tweaks

* Wip on enhancing matching between messages

* Simulation sound explorations.

* Defining intermediate universe states for ping/pong simulation relation

* Simulation relation for ping/pong, working through simulation proof.

* Working simulation proof for pingpong, modulo action matches work

* Code reorganization to help support real adversary simulation proof.

* Preparing for adversarial reasoning in PingPong protocol

* Address review comments and remove tactic debugging from EncPingProtocol

KeyManagement/Common.v
@@ -5,32 +5,125 @@ Set Implicit Arguments.
 Definition user_id              := nat.
 Definition user_list (A : Type) := list (user_id * A).
 
-Fixpoint updateUserList {V : Type} (usrs : user_list V) (u : user_id) (u_d : V) :=
-  match usrs with
-  | (k,v) :: usrs' => if k ==n u
-                     then (u,u_d) :: usrs' (* Case we are interested in *)
-                     else (k,v)   :: updateUserList usrs' u u_d
-  | []             => [(u,u_d)]
-  end.
+Definition updF {V : Type} (u : user_id) (v : V) : nat * V -> nat * V :=
+  fun p => let '(u',v') := p in (u', if u ==n u' then v else v').
 
-Theorem update_inserted:
-  forall V (users users' : user_list V) u_id v,
-    updateUserList users u_id v = users'
-    -> In (u_id,v) users'.
+Definition updateUserList {V : Type} (usrs : user_list V) (u : user_id) (u_d : V) : user_list V :=
+  map (updF u u_d) usrs.
+
+Lemma update_inserted :
+  forall {V} u_id v v' (usrs : user_list V),
+        In (u_id,v)  usrs
+      -> In (u_id,v') (updateUserList usrs u_id v').
 Proof.
-  induct users; intros.
-  - unfold updateUserList in H. invert H. apply in_eq.
-  - destruct a. simpl in *. cases (u_id ==n u). simpl.
-    + rewrite e in *. rewrite <- H. cases (u ==n u); auto using in_eq. destruct n. trivial.
-    + cases (u ==n u_id).
-      * rewrite e in n. destruct n. trivial.
-      * destruct users'.
-        invert H.
-        apply in_cons. apply IHusers. inversion H. trivial.
+  intros.
+  assert (FX: (updF u_id v') (u_id,v) = (u_id,v'))
+    by (simpl; cases (u_id ==n u_id); [reflexivity | contradiction]).
+  rewrite <- FX.
+  unfold updateUserList.
+  eapply in_map; eauto.
 Qed.
 
+Definition keys_uniq {V} (usrs : user_list V) : Prop :=
+  forall k v,
+    In (k,v) usrs
+    -> forall v', In (k,v') usrs
+            -> v = v'.
 
-Print eq_nat_dec.
+Lemma keys_uniq_in :
+  forall {V} k v (usrs : user_list V),
+    In (k,v) usrs
+    -> keys_uniq usrs
+    -> exists l1 l2,
+        usrs = l1 ++ (k,v) :: l2
+        /\ (forall v', In (k,v') l1 -> v = v')
+        /\ (forall v', In (k,v') l2 -> v = v').
+Proof.
+  intros.
+
+  pose proof (in_split (k,v) usrs H) as IN.
+  destruct IN as [l1 IN]. destruct IN as [l2 IN].
+  exists l1. exists l2.
+  unfold keys_uniq in H0.
+  propositional; eauto.
+
+  eapply H0; eauto. rewrite IN. eapply in_or_app; eauto.
+  eapply H0; eauto. rewrite IN. eapply in_or_app. right. eapply in_cons; eauto.
+Qed.
+
+Lemma in_then_same :
+  forall {V} k v (l : user_list V),
+    (forall v', In (k, v') l -> v = v')
+    -> map (updF k v) l = l.
+Proof.
+  intros.
+  induct l; auto; simpl.
+
+  destruct a as [k' v'].
+
+  unfold updF at 1. cases (k ==n k').
+  rewrite e in H.
+  pose proof (H v') as CONTRA. simpl in CONTRA. destruct CONTRA; eauto.
+  rewrite IHl; eauto. rewrite e.
+  intros.
+  eapply H; simpl; eauto.
+
+  simpl in H.
+  rewrite IHl; eauto.
+Qed.
+
+Lemma update_identity_idem :
+  forall {V} u_id v (usrs : user_list V),
+      keys_uniq usrs
+    -> In (u_id,v) usrs
+    -> usrs = updateUserList usrs u_id v.
+Proof.
+  intros.
+  unfold updateUserList.
+
+  pose proof (keys_uniq_in u_id v H0 H).
+  destruct H1 as [l1].
+  destruct H1 as [l2].
+  destruct H1.
+  destruct H2.
+  rewrite H1.
+  rewrite map_app; simpl.
+  cases (u_id ==n u_id); swap 1 2. contradiction.
+  rewrite (in_then_same); eauto.
+  rewrite (in_then_same); eauto.
+Qed.
+
+(* Syntactic type of types for messages *)
+Inductive type :=
+| Nat : type
+| Unit : type
+(* We will definitely need Text, but do we also need special
+ * types for, say, keys.  If so, then we most definitely need
+ * type to be implemented separately for both Real and Ideal worlds.
+ *
+ * | Text : type
+ *)
+| Prod (t1 t2 : type) : type
+.
+
+Fixpoint typeDenote (t : type) : Set :=
+  match t with
+  | Nat  => nat
+  | Unit => unit
+  | Prod t1 t2 => typeDenote t1 * typeDenote t2
+  end.
+
+
+
+(* Exisistential wrapper for stuff, so we can put it in collections *)
+Inductive exmsg : Type :=
+| Exm {A : Type} (wrapped : A) : exmsg.
+
+(* Labels for the labeled transition system *)
+Inductive label  {A} : Type :=
+  Silent : label
+| Action :  A -> label
+.
 
 Lemma pair_uneq_if_fst_uneq:
   forall {A: Type} (p1 p2 : (user_id * A)) ineq,
