KeyManagement/RealWorld.v
@@ -23,76 +23,129 @@ Inductive key :=
 | AsymKey  (k : cryptographic_key) (has_private_access : bool)
 .
 
-(** How are we going to model encryption / decryption in this framework?  Each key has
-    associated with it either:
-    - a key id (in the case of a symmetric key)
-    - a public/privite key pair (in the case of an asymmetric key)
+Definition keyId (k : key) :=
+  match k with
+  | SymKey  ck   => ck.(key_id)
+  | AsymKey ck _ => ck.(key_id)
+  end.
 
-    In order for us to share a secret, we need to appropriately hide that secret so that
-    it cannot be viewed by eavesdroppers.  At the same time, for the purposes of this model
-    we are creating, we need to be able to detect very simply whether a decryption has been
-    successful.  The way we are going to do this, conceptually, is to include the key_id as
-    part of the message, and have the decryption step relation check whether that key_id
-    exists in the user's key heap.  Let's work out more precisely what happens in the two
-    cases:  symmetric and asymmetric keys.
-   
-    * Symmetric Key encryption / decryption
+Definition keyUsage (k : key) :=
+  match k with
+  | SymKey  ck   => ck.(usage)
+  | AsymKey ck _ => ck.(usage)
+  end.
 
-    If I want to encrypt something and share it with someone else using a symmetric key, we
-    first have to generate the key and securely share it.  Ignoring things like usage and
-    the actual sharing process, the steps are:
-    - Generate symmetric key: private_key : symmetric_key := k (system adds to user's key heap)
-    - Securely share k (via Sym_Key_Msg, system adds to user's key heap)
-    - Sending user encrypts with k
-    - Sending user sends encrypted message to receiving user
-    - Receiving user decrypts with k (system verifies k is in decrypting user's key heap)
 
-    * Asymmetric Key encryption / decryption
-
-    Sharing a secret via asymmetric keys has a few more steps, but no 'magical' ones.  Each
-    user generates public/private key pairs, exchange the public parts, and encrypts with
-    a combination of own private key / destination user's public key.  The steps in more
-    detail:
-    - UserA generates key:
-        (pub_key_id, priv_key_id) : (nat,nat) := (pubIdA,privIdA)
-    - UserB generates key:
-        (pub_key_id, priv_key_id) : (nat,nat) := (pubIdB,privIdB)
-    - UserA publicly sends to UserB pubIdA
-    - UserB publicly sends to UserA pubIdB
-    - UserA encrypts message with pubIdB, sends to UserB
-    - UserB decrypts reeived message with privIdB
- *)
-
-(* Messages ultimately wrap either a string or a key 
-   Messages can be encrypted, signed, or HMACed in a nested fashion any number of times 
-   Note: the key_pair_message constructor is temporary and will be removed *)
-Inductive message : Set -> Type :=
-(* Base Message Types *)
-| Plaintext {A : Set} (txt : A) : message A
-| KeyMessage  (k : key) : message key
-
-| MsgPair {A B : Set} (msg1 : message A) (msg2 : message B) : message (A*B)
-
-(* TODO tbraje: is there a way to collapse these two?? *)
-| Ciphertext (msg_id : cipher_id) : message cipher_id
-| Signature  (sig_id : cipher_id) : message cipher_id
+Inductive type :=
+| Nat
+(* | Text *)
+| Key
+| CipherId
+| Pair (t1 t2 : type)
 .
+
+Fixpoint typeDenote (t : type) : Set :=
+  match t with
+  | Nat => nat
+  | Key => key
+  | CipherId => cipher_id
+  | Pair t1 t2 => typeDenote t1 * typeDenote t2
+  end.
+
+Inductive message : type -> Type :=
+(* This will eventually be a message Text, using nat for now *)
+| Plaintext (txt : nat) : message Nat
+| KeyMessage  (k : key) : message Key
+
+| MsgPair {t1 t2 : type} (msg1 : message t1) (msg2 : message t2) : message (Pair t1 t2)
+
+| Ciphertext (msg_id : cipher_id) : message CipherId
+| Signature {t} (msg : message t) (sig : cipher_id) : message (Pair t CipherId)
+.
+
+(* We need to handle non-deterministic message  -- external choice on ordering *)
+Inductive msg_pat :=
+| Accept
+| Paired (pat1 pat2 : msg_pat)
+| Signed (k : key_identifier) (pat : msg_pat)
+| Encrypted (k : key_identifier) (pat : msg_pat)
+.
+
+Inductive cipher : Type :=
+| Cipher {t} (c_id : cipher_id) (k_id : key_identifier) (msg : message t) : cipher
+.
+
+Definition queued_messages := fmap user_id (list exmsg).
+Definition keys            := fmap key_identifier key.
+Definition ciphers         := fmap cipher_id cipher.
+
+Definition adversary_knowledge := keys.
+
+Fixpoint msg_accepted_by_pattern {t} (cs : ciphers) (pat : msg_pat) (msg : message t) : bool :=
+  match pat, msg with
+  | Accept, _ => true
+  | Paired p1 p2, MsgPair m1 m2 => msg_accepted_by_pattern cs p1 m1 && msg_accepted_by_pattern cs p2 m2
+  | Paired _ _, _ => false
+  | Signed k p, Signature _ c_id =>
+    match cs $? c_id with
+    | Some (Cipher _ k_id m) => if (k ==n k_id) then (msg_accepted_by_pattern cs p m) else false
+    | None => false
+    end
+  | Signed _ _, _ => false
+  | Encrypted k p, Ciphertext c_id =>
+    match cs $? c_id with
+    | Some (Cipher _ k_id m) => if (k ==n k_id) then (msg_accepted_by_pattern cs p m) else false
+    | None => false
+    end
+  | Encrypted _ _, _ => false
+  end.
+
+Fixpoint msg_pattern_spoofable (advk : adversary_knowledge) (pat : msg_pat) : bool :=
+  match pat with
+  | Accept => true
+  | Paired p1 p2 => msg_pattern_spoofable advk p1 && msg_pattern_spoofable advk p2
+  | Signed k p =>
+    match advk $? k with
+    | Some _ => msg_pattern_spoofable advk p
+    | None   => false
+    end
+  | Encrypted k p =>
+    match advk $? k with
+    | Some _ => msg_pattern_spoofable advk p
+    | None   => false
+    end
+  end.
+
+Fixpoint msg_spoofable {t} (cs : ciphers) (advk : adversary_knowledge) (msg : message t) : bool :=
+  match msg with
+  | Plaintext _ => true
+  | KeyMessage _ => true
+  | MsgPair m1 m2 => msg_spoofable cs advk m1 && msg_spoofable cs advk m2
+  | Ciphertext c_id => true (* TODO -- how should we actually handle this?? *)
+  | Signature m c_id =>
+    match cs $? c_id with
+    | Some (Cipher _ k_id _) => match advk $? k_id with | Some _ => true | None => false end
+    | None => false
+    end
+  end.
 
 Inductive user_cmd : Type -> Type :=
 (* Plumbing *)
 | Return {A : Type} (res : A) : user_cmd A
 | Bind {A A' : Type} (cmd1 : user_cmd A') (cmd2 : A' -> user_cmd A) : user_cmd A
 
+| Gen : user_cmd nat
+
 (* Messaging *)
-| Send {A : Set} (uid : user_id) (msg : message A) : user_cmd unit
-| Recv {A : Set}: user_cmd (message A)
+| Send {t} (uid : user_id) (msg : message t) : user_cmd unit
+| Recv {t} (pat : msg_pat) : user_cmd (message t)
 
 (* Crypto!! *)
-| Encrypt {A : Set} (k : key) (msg : message A) : user_cmd (message cipher_id)
-| Decrypt {A : Set} (msg : message cipher_id) : user_cmd (message A)
+| Encrypt {t} (k : key) (msg : message t) : user_cmd (message CipherId)
+| Decrypt {t} (msg : message CipherId) : user_cmd (message t)
 
-| Sign    {A : Set} (k : key) (msg : message A) : user_cmd (message cipher_id)
-| Verify  (msg : message cipher_id) : user_cmd bool
+| Sign    {t} (k : key) (msg : message t) : user_cmd (message (Pair t CipherId))
+| Verify  {t} (k : key) (msg : message (Pair t CipherId)) : user_cmd bool
 
 | GenerateSymKey  (usage : key_usage) : user_cmd key
 | GenerateAsymKey (usage : key_usage) : user_cmd key
@@ -109,41 +162,26 @@ End RealWorldNotations.
 Import  RealWorldNotations.
 Open Scope realworld_scope.
 
-(* Exisistential wrapper for message, so we can put it in collections *)
-(* This feels overly complicated to me... *) 
-Inductive exmsg : Type :=
-| Exm {A : Set} (msg : message A) : exmsg.
-
-Check ($0 $+ (1, Exm (Plaintext "foo")) $+ (2, Exm (Plaintext 1))).
-
 Record user_data (A : Type) :=
   mkUserData {
-      usrid    : user_id ;
       key_heap : fmap nat key ;
       protocol : user_cmd A ;
       (* msg_heap : user_msg_heap ; *)
       (* is_admin : bool *)
     }.
 
-Inductive cipher : Type :=
-| Cipher {A: Set} (c_id : cipher_id) (k_id : key_identifier) (msg : message A) : cipher
-.
-
-Definition queued_messages := fmap user_id (list exmsg).
-Definition keys            := fmap key_identifier key.
-Definition ciphers         := fmap cipher_id cipher.
-
 Record universe (A : Type) :=
   mkUniverse {
       users            : user_list (user_data A) ;
       users_msg_buffer : queued_messages ;
       all_keys         : keys ;
-      all_ciphers      : ciphers
+      all_ciphers      : ciphers ;
+      adversary        : adversary_knowledge
     }.
 
 (* This is horribly inefficient, but I want the list to act like a queue.  We want
  * first in - first out semantics to keep message order preserved *)
-Local Definition multiMapAdd {K V} (k : K)(v : V)(m : fmap K (list V)) : fmap K (list V) :=
+Definition multiMapAdd {K V} (k : K)(v : V)(m : fmap K (list V)) : fmap K (list V) :=
   match m $? k with
   | None => m $+ (k, [v])
   | Some vs => m $+ (k, vs ++ [v]) (* add new element to end, to preserve order *)
@@ -152,18 +190,18 @@ Local Definition multiMapAdd {K V} (k : K)(v : V)(m : fmap K (list V)) : fmap K 
 (* When we are finding keys, we need to check whether they are asymmetric.  If
    so, we mark them as not having access to the private key, since the intent is to
    send only the public part of the key *)
-Local Fixpoint findKeys {A} (msg : message A) : list key :=
+Fixpoint findKeys {t} (msg : message t) : list key :=
   match msg with
-  | Plaintext pt       => []
+  | Plaintext _        => []
 
   | KeyMessage (AsymKey k' _) => [AsymKey k' false] (* Only sending public keys *)
   | KeyMessage k       => [k]
   | MsgPair msg1 msg2  => findKeys msg1 ++ findKeys msg2
   | Ciphertext _       => []
-  | Signature _        => []
+  | Signature m _      => findKeys m
   end.
 
-Local Definition updateKeyHeap (ks : list key) (key_heap : keys) : keys :=
+Definition updateKeyHeap (ks : list key) (key_heap : keys) : keys :=
   let addKey (m : keys) (k : key) :=
       match k with
       | SymKey k'     => m $+ (k'.(key_id), k)
@@ -171,13 +209,7 @@ Local Definition updateKeyHeap (ks : list key) (key_heap : keys) : keys :=
       end
   in  fold_left addKey ks key_heap.
 
-Local Definition updateUserKeyHeap {A : Set} (ks : list key) (ud : user_data A) : user_data A :=
-  {| usrid    := ud.(usrid)
-     ; key_heap := updateKeyHeap ks ud.(key_heap)
-     ; protocol := ud.(protocol)
-  |}.
-
-Definition encryptMessage {A} (k : key) (m : message A) (c_id : cipher_id) : option cipher :=
+Definition encryptMessage {t} (k : key) (m : message t) (c_id : cipher_id) : option cipher :=
   match k with
   | SymKey k'  =>
     match (usage k') with
@@ -191,7 +223,7 @@ Definition encryptMessage {A} (k : key) (m : message A) (c_id : cipher_id) : opt
     end
   end.
 
-Definition signMessage {A} (k : key) (m : message A) (c_id : cipher_id) : option cipher :=
+Definition signMessage {t} (k : key) (m : message t) (c_id : cipher_id) : option cipher :=
   match k with
   | SymKey k'  =>
     match (usage k') with
@@ -207,76 +239,155 @@ Definition signMessage {A} (k : key) (m : message A) (c_id : cipher_id) : option
   end.
 
 Definition canVerifySignature {A} (ciphers : fmap cipher_id cipher)(usrDat : user_data A)(c_id : cipher_id) : Prop :=
-  forall (M : Set) (m : message M) k_id k ,
+  forall t (m : message t) k_id k ,
     ciphers $? c_id = Some (Cipher c_id k_id m)
     (*  Make sure that the user has access to the key.  If we are doing asymmetric signatures,
         we only need the public part of the key, so no additional checks necessary! *)
     /\ usrDat.(key_heap) $? k_id = Some k.
 
 Definition data_step0 (A : Type) : Type := 
-  ciphers * keys * queued_messages * fmap nat key * user_cmd A.
+  adversary_knowledge * ciphers * keys * queued_messages * fmap nat key * user_cmd A.
 
-Inductive step_user : forall A, user_id -> data_step0 A -> data_step0 A -> Prop :=
+Definition updateUniverse {A} (U : universe A) (advk : adversary_knowledge) (cs : ciphers)
+                          (ks : keys) (qmsgs : queued_messages)
+                          (u_id : user_id) (userKeys : keys) (cmd : user_cmd A): universe A :=
+  {|
+    users            := updateUserList U.(users) u_id ( mkUserData userKeys cmd )
+  ; users_msg_buffer := qmsgs
+  ; all_keys         := ks
+  ; all_ciphers      := cs
+  ; adversary        := advk
+  |}.
+
+Definition addUniverseUsers {A} (U : universe A) (adversaries : user_list (user_data A)) :=
+  {|
+    users            := U.(users) ++ adversaries
+  ; users_msg_buffer := U.(users_msg_buffer)
+  ; all_keys         := U.(all_keys)
+  ; all_ciphers      := U.(all_ciphers)
+  ; adversary        := U.(adversary)
+  |}.
+
+Definition extractPlainText {t} (msg : message t) : option nat :=
+  match msg with
+  | Plaintext t => Some t
+  | _           => None
+  end.
+
+Definition unPair {t1 t2} (msg : message (Pair t1 t2)) : option (message t1 * message t2)  :=
+  match msg
+        in (message t)
+        (* return (match t with _ => option (message t1 * message t2) end) *)
+        return (match t with
+                | Pair t1 t2 => option (message t1 * message t2)
+                | _ => option (message t1 * message t2) end)
+  with
+  | MsgPair m1 m2 => Some (m1,m2)
+  | _             => None
+  end.
+
+
+(* The Operational Semantics we want --> a labeled transition system *)
+
+Inductive action : Type :=
+| Input  t (msg : message t) (pat : msg_pat) (u_id : user_id) (uks : keys) (cs : ciphers)
+| Output t (msg : message t) (u_id : user_id)
+.
+
+Definition rlabel := @label action.
+
+Definition action_adversary_safe (advk : adversary_knowledge) (a : action) : bool :=
+  match a with
+  | Input _ pat _ _ _ => negb (msg_pattern_spoofable advk pat)
+  | Output _ _        => true
+  end.
+
+Definition universe_data_step {A} (U : universe A) (u_data : user_data A) : data_step0 A :=
+  (U.(adversary), U.(all_ciphers), U.(all_keys), U.(users_msg_buffer), u_data.(key_heap), u_data.(protocol)).
+
+(* Labeled transition system *)
+Inductive lstep_user : forall A, user_id -> rlabel -> data_step0 A -> data_step0 A -> Prop := 
 
 (* Plumbing *)
-| StepBindRecur : forall {r r'} u_id cs cs' ks ks' msgs msgs' uks uks' (cmd1 cmd1' : user_cmd r) (cmd2 : r -> user_cmd r'),
-    step_user u_id (cs, ks, msgs, uks, cmd1) (cs', ks', msgs', uks', cmd1')
-    -> step_user u_id (cs, ks, msgs, uks, Bind cmd1 cmd2) (cs', ks', msgs', uks', Bind cmd1' cmd2)
-| StepBindProceed : forall {r r'} u_id cs ks msgs uks (v : r') (cmd : r' -> user_cmd r),
-    step_user u_id (cs, ks, msgs, uks, Bind (Return v) cmd) (cs, ks, msgs, uks, cmd v)
+| LStepBindRecur : forall {r r'} u_id advk advk'
+                     cs cs' ks ks' msgs msgs'
+                     uks uks' lbl (cmd1 cmd1' : user_cmd r) (cmd2 : r -> user_cmd r'),
+      lstep_user u_id lbl (advk, cs, ks, msgs, uks, cmd1) (advk', cs', ks', msgs', uks', cmd1')
+    -> lstep_user u_id lbl (advk, cs, ks, msgs, uks, Bind cmd1 cmd2) (advk', cs', ks', msgs', uks', Bind cmd1' cmd2)
+| LStepBindProceed : forall {r r'} u_id advk cs ks msgs uks (v : r') (cmd : r' -> user_cmd r),
+    lstep_user u_id Silent (advk, cs, ks, msgs, uks, Bind (Return v) cmd) (advk, cs, ks, msgs, uks, cmd v)
 
-(* Comms *)
-| StepRecv : forall {A} u_id cs ks qmsgs qmsgs' uks (msg : message A) msgs newkeys,
+| LGen : forall u_id advk cs ks msgs uks n,
+    lstep_user u_id Silent (advk, cs, ks, msgs, uks, Gen) (advk, cs, ks, msgs, uks, Return n)
+
+(* Comms  *)
+| LStepRecv : forall {t} u_id advk cs ks qmsgs qmsgs' uks (msg : message t) pat msgs newkeys,
     qmsgs $? u_id = Some (Exm msg :: msgs) (* we have a message waiting for us! *)
     -> qmsgs' = match msgs with [] => qmsgs $- u_id | _ => qmsgs $+ (u_id,msgs) end
     -> findKeys msg = newkeys
-    -> step_user u_id (cs, ks, qmsgs, uks, Recv)
-                     (cs, ks, qmsgs', updateKeyHeap newkeys uks, Return msg)
-| StepSend : forall {A} u_id cs ks qmsgs rec_u_id uks (msg : message A),
-    step_user u_id (cs, ks, qmsgs, uks, Send rec_u_id msg)
-                   (cs, ks, multiMapAdd rec_u_id (Exm msg) qmsgs, uks, Return tt)
+    -> msg_accepted_by_pattern cs pat msg = true
+    -> lstep_user u_id (Action (Input msg pat u_id uks cs))
+                 (advk, cs, ks, qmsgs, uks, Recv pat)
+                 (advk, cs, ks, qmsgs', updateKeyHeap newkeys uks, Return msg)
+
+| LStepRecvDrop : forall {t} u_id advk cs ks qmsgs qmsgs' uks (msg : message t) pat msgs,
+      qmsgs $? u_id = Some (Exm msg :: msgs) (* we have a message waiting for us! *)
+    -> qmsgs' = match msgs with [] => qmsgs $- u_id | _ => qmsgs $+ (u_id,msgs) end
+    (* Hrm, when I am dropping the message, do I want to process keys?? *)
+    (* -> findKeys msg = newkeys *)
+    -> msg_accepted_by_pattern cs pat msg = false
+    -> lstep_user u_id Silent (* Error label ... *)
+                 (advk, cs, ks, qmsgs,  uks, @Recv t pat)
+                 (advk, cs, ks, qmsgs', uks, Recv pat)
+
+(* Augment attacker's keys with those available through messages sent, including traversing through ciphers already known by attacker, etc. *)
+| LStepSend : forall {t} u_id advk advk' cs ks qmsgs rec_u_id uks newkeys (msg : message t),
+    findKeys msg = newkeys
+    -> advk' = updateKeyHeap newkeys advk
+    -> lstep_user u_id (Action (Output msg u_id))
+               (advk,  cs, ks, qmsgs, uks, Send rec_u_id msg)
+               (advk', cs, ks, multiMapAdd rec_u_id (Exm msg) qmsgs, uks, Return tt)
 
 (* Encryption / Decryption *)
-(* | StepEncrypt : forall {A} cs ks qmsgs usrDat (msg : message A) k k_id c_id cipherMsg, *)
-(*     usrDat.(key_heap) $? k_id = Some k *)
-(*     -> ~(c_id \in (dom cs)) *)
-(*     -> encryptMessage k msg c_id = Some cipherMsg *)
-(*     -> step_user (cs, ks, qmsgs, usrDat, Encrypt k msg) *)
-(*                 (cs $+ (c_id, cipherMsg), ks, qmsgs, usrDat, Return (Ciphertext c_id)) *)
+| LStepEncrypt : forall {t} u_id advk cs ks qmsgs uks (msg : message t) k k_id c_id cipherMsg,
+    keyId k = k_id
+    -> uks $? k_id = Some k
+    -> ~(c_id \in (dom cs))
+    -> encryptMessage k msg c_id = Some cipherMsg
+    -> lstep_user u_id Silent
+                 (advk, cs, ks, qmsgs, uks, Encrypt k msg)
+                 (advk, cs $+ (c_id, cipherMsg), ks, qmsgs, uks, Return (Ciphertext c_id))
 
-(* | StepSymmetricDecrypt : forall {A} cs ks qmsgs usrDat (msg : message A) k_id k c_id newkeys, *)
-(*     cs $? c_id = Some (Cipher c_id k_id msg) *)
-(*     -> usrDat.(key_heap) $? k_id = Some (SymKey k) *)
-(*     -> findKeys msg = newkeys (* find keys in new key heap *) *)
-(*     -> step_user (cs, ks, qmsgs, usrDat, Decrypt (Ciphertext c_id)) *)
-(*                 (cs, ks, qmsgs, updateUserKeyHeap newkeys usrDat, Return msg) *)
-
-(* | StepAsymmetricDecrypt : forall {A} cs ks qmsgs usrDat (msg : message A) k_id k c_id newkeys, *)
-(*     cs $? c_id = Some (Cipher c_id k_id msg) *)
-(*     -> usrDat.(key_heap) $? k_id = Some (AsymKey k true) (* check we have access to private key *) *)
-(*     -> findKeys msg = newkeys *)
-(*     -> step_user (cs, ks, qmsgs, usrDat, Decrypt (Ciphertext c_id)) *)
-(*                 (cs, ks, qmsgs, updateUserKeyHeap newkeys usrDat, Return msg) *)
+| LStepDecrypt : forall {t} u_id advk cs ks qmsgs uks (msg : message t) k_id k c_id newkeys,
+    cs $? c_id = Some (Cipher c_id k_id msg)
+    -> ( uks $? k_id = Some (AsymKey k true) (* check we have access to private key *)
+      \/ uks $? k_id = Some (SymKey k) )
+    -> k.(key_id) = k_id
+    -> findKeys msg = newkeys
+    -> lstep_user u_id Silent
+                 (advk, cs, ks, qmsgs, uks, Decrypt (Ciphertext c_id))
+                 (advk, cs, ks, qmsgs, updateKeyHeap newkeys uks, Return msg)
 
 (* Signing / Verification *)
-(* | StepSign : forall {A} cs ks qmsgs usrDat k_id k (msg : message A) c_id cipherMsg, *)
-(*     usrDat.(key_heap) $? k_id = Some k *)
-(*     -> ~(c_id \in (dom cs)) *)
-(*     -> signMessage k msg c_id = Some cipherMsg *)
-(*     -> step_user (cs, ks, qmsgs, usrDat, Sign k msg) *)
-(*                 (cs $+ (c_id, cipherMsg), ks, qmsgs, usrDat, Return (Signature c_id)) *)
-(* | StepVerify : forall cs ks qmsgs usrDat c_id, *)
-(*     canVerifySignature cs usrDat c_id *)
-(*     -> step_user (cs, ks, qmsgs, usrDat, Verify (Signature c_id)) *)
-(*                 (cs, ks, qmsgs, usrDat, Return true) *)
-(* | StepFailVerify : forall cs ks qmsgs usrDat c_id, *)
-(*     ~ canVerifySignature cs usrDat c_id *)
-(*     -> step_user (cs, ks, qmsgs, usrDat, Verify (Signature c_id)) *)
-(*                 (cs, ks, qmsgs, usrDat, Return false) *)
-(* | StepFailVerifyNotSig : forall cs ks qmsgs usrDat c_id msg, *)
-(*     ~ msg <> Signature c_id *)
-(*     -> step_user (cs, ks, qmsgs, usrDat, Verify msg) *)
-(*                 (cs, ks, qmsgs, usrDat, Return false) *)
+| LStepSign : forall {t} u_id advk cs ks qmsgs uks (msg : message t) k k_id c_id cipherMsg,
+      keyId k = k_id
+    -> uks $? k_id = Some k
+    -> ~(c_id \in (dom cs))
+    -> signMessage k msg c_id = Some cipherMsg
+    -> lstep_user u_id Silent
+                 (advk, cs, ks, qmsgs, uks, Sign k msg)
+                 (advk, cs $+ (c_id, cipherMsg), ks, qmsgs, uks, Return (Signature msg c_id))
+
+| LStepVerify : forall {t} u_id advk cs ks qmsgs uks (msg : message t) k_id k c_id newkeys,
+    (* k is in your key heap *)
+    uks $? (keyId k) = Some k
+    (* return true or false whether k was used to sign the message *)
+    -> cs $? c_id = Some (Cipher c_id k_id msg)
+    -> findKeys msg = newkeys (* TODO do we really want this, should have been gotten via recieve???  find keys that might be in message *)
+    -> lstep_user u_id Silent
+                 (advk, cs, ks, qmsgs, uks, (Verify k (MsgPair msg (Ciphertext c_id))))
+                 (advk, cs, ks, qmsgs, updateKeyHeap newkeys uks, Return (if (k_id ==n (keyId k)) then true else false))
+.
 
 (* Key creation *)
 (* | StepGenerateSymKey: forall A cs ks qmsgs (usrDat : user_data A) usage k kid, *)
@@ -291,88 +402,47 @@ Inductive step_user : forall A, user_id -> data_step0 A -> data_step0 A -> Prop 
 (*                 (cs, ks $+ (kid, k), qmsgs, updateUserKeyHeap [k] usrDat, Return k) *)
                 
 (* | Barrier {result : Set} : user_cmd result. *)
-.
 
-Lemma StepRecv' : forall {A} u_id cs ks qmsgs qmsgs' uks uks' (msg : message A) msgs newkeys,
+Lemma LStepRecv' : forall {t} u_id advk cs ks qmsgs qmsgs' uks uks' (msg : message t) pat msgs newkeys,
   qmsgs $? u_id = Some (Exm msg :: msgs) (* we have a message waiting for us! *)
   -> qmsgs' = match msgs with [] => qmsgs $- u_id | _ => qmsgs $+ (u_id,msgs) end
+  -> msg_accepted_by_pattern cs pat msg = true
   -> findKeys msg = newkeys
   -> uks' = updateKeyHeap newkeys uks
-  -> step_user u_id (cs, ks, qmsgs, uks, Recv)
-                        (cs, ks, qmsgs', uks', Return msg).
+  -> lstep_user u_id (Action (Input msg pat u_id uks cs))
+               (advk, cs, ks, qmsgs,  uks,  Recv pat)
+               (advk, cs, ks, qmsgs', uks', Return msg).
 Proof.
   intros. subst. econstructor; eauto.
 Qed.
 
-Definition updateUniverse {A} (U : universe A) (cs : ciphers) (ks : keys) (qmsgs : queued_messages)
-                          (u_id : user_id) (userKeys : keys) (cmd : user_cmd A): universe A :=
-  {|
-    users            := updateUserList U.(users) u_id ( mkUserData u_id userKeys cmd )
-  ; users_msg_buffer := qmsgs
-  ; all_keys         := ks
-  ; all_ciphers      := cs
-  |}.
+Lemma LStepRecvDrop' : forall {t} u_id advk cs ks qmsgs qmsgs' uks (msg : message t) pat msgs,
+  qmsgs $? u_id = Some (Exm msg :: msgs) (* we have a message waiting for us! *)
+  -> qmsgs' = match msgs with [] => qmsgs $- u_id | _ => qmsgs $+ (u_id,msgs) end
+  -> msg_accepted_by_pattern cs pat msg = false
+  -> lstep_user u_id Silent
+               (advk, cs, ks, qmsgs,  uks, @Recv t pat)
+               (advk, cs, ks, qmsgs', uks, Recv pat).
+Proof.
+  intros. subst. econstructor; eauto.
+Qed.
 
-Inductive step_universe {A} : universe A -> universe A -> Prop :=
-| StepUser : forall U u_id userData uks cs ks qmsgs (cmd' : user_cmd A),
+Inductive lstep_universe {A} : universe A -> rlabel -> universe A -> Prop :=
+| LStepUser : forall U u_id userData uks advk cs ks qmsgs lbl (cmd' : user_cmd A),
     In (u_id,userData) U.(users)
-    (* U.(users) $? u_id = Some userData *)
-    -> step_user u_id (U.(all_ciphers), U.(all_keys), U.(users_msg_buffer), userData.(key_heap), userData.(protocol))
-                     (cs, ks, qmsgs, uks, cmd')
-    -> step_universe U (updateUniverse U cs ks qmsgs u_id uks cmd')
+    -> lstep_user u_id lbl
+                 (universe_data_step U userData)
+                 (advk, cs, ks, qmsgs, uks, cmd')
+    -> lstep_universe U lbl (updateUniverse U advk cs ks qmsgs u_id uks cmd')
 .
 
-
-Lemma StepUser' : forall A U U' u_id userData uks cs ks qmsgs ( cmd' : user_cmd A),
+Lemma LStepUser' : forall A U U' u_id userData uks advk cs ks qmsgs lbl ( cmd' : user_cmd A),
   In (u_id,userData) U.(users)
-  (* U.(users) $? u_id = Some userData *)
-  -> step_user u_id (U.(all_ciphers), U.(all_keys), U.(users_msg_buffer), userData.(key_heap), userData.(protocol))
-                        (cs, ks, qmsgs, uks, cmd')
-  -> U' = (updateUniverse U cs ks qmsgs u_id uks cmd')
-  -> step_universe U U'.
+  -> lstep_user u_id lbl
+               (universe_data_step U userData)
+               (advk, cs, ks, qmsgs, uks, cmd')
+  -> U' = (updateUniverse U advk cs ks qmsgs u_id uks cmd')
+  -> lstep_universe U lbl U'.
 Proof.
   intros. subst. econstructor; eassumption.
 Qed.
-
-
-Definition extractPlainText {A} (msg : message A) : option A :=
-  match msg with
-  | Plaintext t => Some t
-  | _           => None
-  end.
-
-Section PingProtocol.
-
-  Example ping : list (user_data nat) :=
-    {| usrid    := 0
-     ; key_heap := $0
-     ; protocol := (  _ <- Send 1 (Plaintext 1)
-                    ; Return 42)
-    |}
-      ::
-    {| usrid    := 1
-     ; key_heap := $0
-     ; protocol := (  rec <- Recv (A := nat)
-                    ; Return (match extractPlainText rec with
-                              | Some msg => msg
-                              | None     => 98
-                              end))
-    |}
-      :: [].
-
-  Example ping_universe : universe nat :=
-    {|
-      users            := map (fun u_d => (u_d.(usrid), u_d)) ping
-    ; users_msg_buffer := $0
-    ; all_keys         := $0
-    ; all_ciphers      := $0
-    |}.
-
-  Check ping_universe.
-
-End PingProtocol.
-
-(* Additional functionality to implement:
-   1. Administration
-   2. CA
-*) 
