KeyManagement/EncPingProtocol.v
@@ -1,0 +1,591 @@
+From Coq Require Import List.
+Require Import Frap.
+
+Require Import Common Simulation.
+Require IdealWorld RealWorld.
+
+Import IdealWorld.IdealNotations.
+Import RealWorld.RealWorldNotations.
+
+Set Implicit Arguments.
+
+(* User ids *)
+Definition A : user_id   := 0.
+Definition B : user_id   := 1.
+Definition ADV : user_id := 2.
+
+Section IdealProtocol.
+  Import IdealWorld.
+
+  Definition CH__A2B : channel_id := 0.
+  Definition CH__B2A : channel_id := 1.
+
+  Definition PERMS__a := $0 $+ (CH__A2B, {| read := false; write := true |}) $+ (CH__B2A, {| read := true; write := false |}).
+  Definition PERMS__b := $0 $+ (CH__B2A, {| read := false; write := true |}) $+ (CH__A2B, {| read := true; write := false |}).
+
+  Definition mkiU (cv : channels) (p__a p__b : cmd bool): universe bool :=
+    {| channel_vector := cv
+     ; users :=
+         [ (A,   {| perms    := PERMS__a ; protocol := p__a |})
+         ; (B,   {| perms    := PERMS__b ; protocol := p__b |})
+         ]
+    |}.
+
+  Definition ideal_univ_start :=
+    mkiU ($0 $+ (CH__A2B, { }) $+ (CH__B2A, { }))
+         ( n <- Gen
+         ; _ <- Send (Content n) CH__A2B
+         ; m <- @Recv Nat CH__B2A
+         ; Return match extractContent m with
+                  | None =>    false
+                  | Some n' => if n ==n n' then true else false
+                  end)
+         ( m <- @Recv Nat CH__A2B
+         ; _ <- Send m CH__B2A
+         ; Return true).
+
+  Definition ideal_univ_sent1 n :=
+    mkiU ($0 $+ (CH__A2B, {Exm (Content n)}) $+ (CH__B2A, { }))
+         ( _ <- Return tt
+         ; m <- @Recv Nat CH__B2A
+         ; Return match extractContent m with
+                  | None =>    false
+                  | Some n' => if n ==n n' then true else false
+                  end)
+         ( m <- @Recv Nat CH__A2B
+         ; _ <- Send m CH__B2A
+         ; Return true).
+
+  Definition ideal_univ_recd1 n :=
+    mkiU ($0 $+ (CH__A2B, {Exm (Content n)}) $+ (CH__B2A, { }))
+         ( m <- @Recv Nat CH__B2A
+         ; Return match extractContent m with
+                  | None =>    false
+                  | Some n' => if n ==n n' then true else false
+                  end)
+         ( m <- Return (Content n)
+         ; _ <- Send m CH__B2A
+         ; Return true).
+
+  Definition ideal_univ_sent2 n :=
+    mkiU ($0 $+ (CH__A2B, {Exm (Content n)}) $+ (CH__B2A, {Exm (Content n)}))
+         ( m <- @Recv Nat CH__B2A
+         ; Return match extractContent m with
+                  | None =>    false
+                  | Some n' => if n ==n n' then true else false
+                  end)
+         ( _ <- Return tt
+         ; Return true).
+
+  Definition ideal_univ_recd2 n :=
+    mkiU ($0 $+ (CH__A2B, {Exm (Content n)}) $+ (CH__B2A, {Exm (Content n)}))
+         ( m <- Return (Content n)
+         ; Return match extractContent m with
+                  | None =>    false
+                  | Some n' => if n ==n n' then true else false
+                  end)
+         (Return true).
+
+  Definition ideal_univ_done n :=
+    mkiU ($0 $+ (CH__A2B, {Exm (Content n)}) $+ (CH__B2A, {Exm (Content n)}))
+         (Return true)
+         (Return true).
+
+End IdealProtocol.
+
+Section RealProtocolParams.
+  Import RealWorld.
+
+  Definition KID1 : key_identifier := 0.
+  Definition KID2 : key_identifier := 1.
+
+  Definition KEY1  := MkCryptoKey KID1 Signing.
+  Definition KEY2  := MkCryptoKey KID2 Signing.
+  Definition KEY__A  := AsymKey KEY1 true.
+  Definition KEY__B  := AsymKey KEY2 true.
+  Definition KEYS  := $0 $+ (KID1, AsymKey KEY1 true) $+ (KID2, AsymKey KEY2 true).
+
+  Definition A__keys := $0 $+ (KID1, AsymKey KEY1 true)  $+ (KID2, AsymKey KEY2 false).
+  Definition B__keys := $0 $+ (KID1, AsymKey KEY1 false) $+ (KID2, AsymKey KEY2 true).
+End RealProtocolParams.
+
+Module Type enemy.
+  Import RealWorld.
+  Parameter code : user_cmd bool.
+End enemy.
+
+Section RealProtocol.
+  Import RealWorld.
+
+  Definition mkrU (usr_msgs : queued_messages) (cs : ciphers) (p__a p__b : user_cmd bool) (adversaries : user_list (user_data bool)) : universe bool :=
+    {| users            :=
+           (A, {| key_heap := A__keys ; protocol := p__a |})
+         :: (B, {| key_heap := B__keys ; protocol := p__b |})
+         :: adversaries
+     ; users_msg_buffer := usr_msgs
+     ; all_keys         := KEYS
+     ; all_ciphers      := cs
+     ; adversary        := $0
+     |}.
+
+  Definition real_univ_start cs :=
+    mkrU $0 cs
+         ( n  <- Gen
+         ; m  <- Sign KEY__A (Plaintext n)
+         ; _  <- Send B m
+         ; m' <- @Recv (Pair Nat CipherId) (Signed KID2 Accept)
+         ; Return match unPair m' with
+                  | Some (Plaintext n', _) => if n ==n n' then true else false (* also do verify? *)
+                  | _ => false
+                  end)
+
+         ( m  <- @Recv (Pair Nat CipherId) (Signed KID1 Accept)
+         ; v  <- Verify (AsymKey KEY1 false) m
+         ; m' <- match unPair m with
+                | Some (p,_) => Sign KEY__B p
+                | Nothing    => Sign KEY__B (Plaintext 1)
+                end
+         ; _  <- Send A m'
+         ; Return v).
+
+  Definition real_univ_sent1 n cs cid1 :=
+    mkrU ($0 $+ (B, [Exm (Signature (Plaintext n) cid1)]))
+         (cs $+ (cid1, Cipher cid1 KID1 (Plaintext n)))
+         ( _  <- Return tt
+         ; m' <- @Recv (Pair Nat CipherId) (Signed KID2 Accept)
+         ; Return match unPair m' with
+                  | Some (Plaintext n', _) => if n ==n n' then true else false (* also do verify? *)
+                  | _ => false
+                  end)
+
+         ( m  <- @Recv (Pair Nat CipherId) (Signed KID1 Accept)
+         ; v  <- Verify (AsymKey KEY1 false) m
+         ; m' <- match unPair m with
+                | Some (p,_) => Sign KEY__B p
+                | Nothing    => Sign KEY__B (Plaintext 1)
+                end
+         ; _  <- Send A m'
+         ; Return v).
+
+  Definition real_univ_recd1 n cs cid1 :=
+    mkrU $0
+         (cs $+ (cid1, Cipher cid1 KID1 (Plaintext n)))
+         ( _  <- Return tt
+         ; m' <- @Recv (Pair Nat CipherId) (Signed KID2 Accept)
+         ; Return match unPair m' with
+                  | Some (Plaintext n', _) => if n ==n n' then true else false (* also do verify? *)
+                  | _ => false
+                  end)
+
+         ( m  <- Return (Signature (Plaintext n) cid1)
+         ; v  <- Verify (AsymKey KEY1 false) m
+         ; m' <- match unPair m with
+                | Some (p,_) => Sign KEY__B p
+                | Nothing    => Sign KEY__B (Plaintext 1)
+                end
+         ; _  <- Send A m'
+         ; Return v).
+
+  Definition real_univ_sent2 n cid1 cid2 :=
+    mkrU ($0 $+ (A, [Exm (Signature (Plaintext n) cid2)]))
+         ($0 $+ (cid1, Cipher cid1 KID1 (Plaintext n)) $+ (cid2, Cipher cid2 KID2 (Plaintext n)))
+         ( _  <- Return tt
+         ; m' <- @Recv (Pair Nat CipherId) (Signed KID2 Accept)
+         ; Return match unPair m' with
+                  | Some (Plaintext n', _) => if n ==n n' then true else false (* also do verify? *)
+                  | _ => false
+                  end)
+
+         ( _  <- Return tt ; Return true).
+
+  Definition real_univ_recd2 n cid1 cid2 :=
+    mkrU $0 ($0 $+ (cid1, Cipher cid1 KID1 (Plaintext n)) $+ (cid2, Cipher cid2 KID2 (Plaintext n)))
+         ( m' <- Return (Signature (Plaintext n) cid2)
+         ; Return match unPair m' with
+                  | Some (Plaintext n', _) => if n ==n n' then true else false (* also do verify? *)
+                  | _ => false
+                  end)
+
+         ( _  <- Return tt ; Return true).
+
+  Definition real_univ_done cs :=
+    mkrU $0 cs (Return true) (Return true).
+
+  Inductive RPingPongBase: RealWorld.universe bool -> IdealWorld.universe bool -> Prop :=
+  | Start : forall U__r cs,
+        rstepSilent^* (real_univ_start cs []) U__r
+      -> RPingPongBase U__r ideal_univ_start
+
+  | Sent1 : forall U__r cs cid1 n,
+        rstepSilent^* (real_univ_sent1 n cs cid1 []) U__r
+      -> RPingPongBase U__r (ideal_univ_sent1 n)
+
+  | Recd1 : forall U__r cs cid1 n,
+        rstepSilent^* (real_univ_recd1 n cs cid1 []) U__r
+      -> RPingPongBase U__r (ideal_univ_recd1 n)
+
+  | Sent2 : forall U__r cid1 cid2 n,
+        rstepSilent^* (real_univ_sent2 n cid1 cid2 []) U__r
+      -> RPingPongBase U__r (ideal_univ_sent2 n)
+
+  | Recd2 : forall U__r cid1 cid2 n,
+        rstepSilent^* (real_univ_recd2 n cid1 cid2 []) U__r
+      -> RPingPongBase U__r (ideal_univ_recd2 n)
+
+  | Done : forall cs n,
+      RPingPongBase (real_univ_done cs []) (ideal_univ_done n)
+  .
+
+End RealProtocol.
+
+Module SimulationAutomation.
+
+  Ltac churn1 :=
+    match goal with
+    | [ H: In _ _ |- _ ] => invert H
+    | [ H : $0 $? _ = Some _ |- _ ] => apply lookup_empty_not_Some in H; contradiction
+    | [ H : _ $? _ = Some _ |- _ ] => apply lookup_split in H; propositional; subst
+    | [ H : (_ $- _) $? _ = Some _ |- _ ] => rewrite addRemoveKey in H by auto
+    | [ H : Some _ = Some _ |- _ ] => invert H
+
+    | [ H : (_ :: _) = _ |- _ ] => invert H
+    | [ H : (_,_) = (_,_) |- _ ] => invert H
+
+    | [ H : updF _ _ _ = _ |- _ ] => unfold updF; simpl in H
+
+    | [ H: RealWorld.Cipher _ _ _ = RealWorld.Cipher _ _ _ |- _ ] => invert H
+    | [ H: RealWorld.SymKey _ = _ |- _ ] => invert H
+    | [ H: RealWorld.AsymKey _ _ = _ |- _ ] => invert H
+
+    | [ H: exists _, _ |- _ ] => invert H
+    | [ H: _ /\ _ |- _ ] => invert H
+
+    (* Only take a user step if we have chosen a user *)
+    | [ H: RealWorld.lstep_user A _ _ _ |- _ ] => invert H
+    | [ H: RealWorld.lstep_user B _ _ _ |- _ ] => invert H
+
+    | [ H: rstepSilent _ _ |- _ ] => invert H (* unfold rstepSilent in H *)
+    | [ H: RealWorld.lstep_universe _ _ _ |- _ ] => invert H
+
+    (* Effectively clears hypotheses of this kind, assuming they are correct.  Otherwise,
+     * I have problems with the automation trying to identify cipher ids. *)
+    | [ H : RealWorld.keyId _ = _ |- _] => invert H
+
+    | [ H: RealWorld.signMessage _ _ _ = _ |- _ ] => unfold RealWorld.encryptMessage; simpl in H
+    | [ H: RealWorld.encryptMessage _ _ _ = _ |- _ ] => unfold RealWorld.encryptMessage; simpl in H
+
+    | [ H: RealWorld.msg_accepted_by_pattern _ _ _ = _ |- _ ] =>
+      unfold RealWorld.msg_accepted_by_pattern in H;
+      rewrite lookup_add_eq in H by eauto;
+      try discriminate
+    (* | [ H : match (_ $+ (_, RealWorld.Cipher _ _ _)) $? _ with _ => _ end = false |- _ ] => *)
+    (*   rewrite lookup_add_eq in H by eauto; try discriminate *)
+    | [ H : RealWorld.msg_spoofable _ _ _ = _ |- _] =>
+      unfold RealWorld.msg_spoofable in H;
+      rewrite lookup_add_eq in H by eauto;
+      simplify;
+      discriminate
+    end.
+
+  Ltac risky1 :=
+    match goal with
+    | [ H: rstepSilent^* _ _ |- _ ] => invert H
+      (* idtac "risk"; (churn1 || idtac "nochurn"); invert H *)
+    end.
+
+  Ltac churn := 
+    repeat (repeat churn1; try risky1; repeat churn1).
+
+  Ltac istep_univ pick :=
+    eapply IdealWorld.LStepUser'; simpl; [ pick; reflexivity | | reflexivity]; simpl.
+
+  Ltac user0 := left.
+  Ltac user1 := right;left.
+
+  Ltac istep_univ0 := istep_univ user0.
+  Ltac istep_univ1 := istep_univ user1.
+
+  Ltac r_single_silent_step :=
+      eapply RealWorld.LStepBindProceed
+    || eapply RealWorld.LGen
+    || eapply RealWorld.LStepRecvDrop
+    || eapply RealWorld.LStepEncrypt
+    || eapply RealWorld.LStepDecrypt
+    || eapply RealWorld.LStepSign
+    || eapply RealWorld.LStepVerify
+  .
+
+  Ltac real_silent_step pick :=
+    eapply TrcFront; [
+      eapply RealWorld.LStepUser'; simpl; [pick; reflexivity | | reflexivity];
+        (eapply RealWorld.LStepBindRecur; r_single_silent_step) || r_single_silent_step
+     |]; simpl.
+
+  Ltac real_silent_step0 := real_silent_step user0.
+  Ltac real_silent_step1 := real_silent_step user1.
+
+  Ltac i_single_silent_step :=
+      eapply IdealWorld.LStepBindProceed
+    || eapply IdealWorld.LStepGen
+    || eapply IdealWorld.LStepCreateChannel
+  .
+
+  Ltac ideal_silent_step pick :=
+    eapply TrcFront; [
+      eapply IdealWorld.LStepUser'; simpl;
+      [ pick; reflexivity | | reflexivity];
+      (eapply IdealWorld.LStepBindRecur; i_single_silent_step) || i_single_silent_step
+     |]; simpl.
+
+  Ltac ideal_silent_step0 := ideal_silent_step user0.
+  Ltac ideal_silent_step1 := ideal_silent_step user1.
+  Ltac ideal_silent_steps := (ideal_silent_step0 || ideal_silent_step1) ; repeat ideal_silent_step0; repeat ideal_silent_step1; eapply TrcRefl.
+
+  Remove Hints TrcRefl TrcFront.
+
+  Hint Constructors RPingPongBase action_matches msg_eq.
+  Hint Resolve IdealWorld.LStepSend' IdealWorld.LStepRecv'.
+
+  Hint Extern 2 (rstepSilent ^* _ _) => (solve [eapply TrcRefl]) || real_silent_step0.
+  Hint Extern 2 (rstepSilent ^* _ _) => (solve [eapply TrcRefl]) || real_silent_step1.
+  Hint Extern 1 (RPingPongBase _ (RealWorld.updateUniverse _ _ _ _ _ _ _ _) _) => unfold RealWorld.updateUniverse; simpl.
+
+  Hint Extern 2 (IdealWorld.lstep_universe _ _ _) => istep_univ0.
+  Hint Extern 2 (IdealWorld.lstep_universe _ _ _) => istep_univ1.
+  Hint Extern 1 (IdealWorld.lstep_user _ (_,(IdealWorld.Bind _ _)%idealworld,_) _) => eapply IdealWorld.LStepBindRecur.
+  Hint Extern 1 (istepSilent ^* _ _) => ideal_silent_steps || apply TrcRefl.
+
+  Hint Extern 1 (In _ _) => progress simpl.
+
+  Hint Extern 1 (RealWorld.encryptMessage _ _ _ = _) => unfold RealWorld.encryptMessage; simpl.
+  Hint Extern 1 (RealWorld.signMessage _ _ _ = _) => unfold RealWorld.signMessage; simpl.
+  Hint Extern 1 (RealWorld.action_adversary_safe _ _ = _) => unfold RealWorld.action_adversary_safe; simplify.
+  Hint Extern 1 (IdealWorld.msg_permissions_valid _ _) => progress simpl.
+
+  Hint Extern 1 (A__keys $? _ = _) => unfold A__keys, B__keys, KEY1, KEY2, KEY__A, KEY__B, KID1, KID2.
+  Hint Extern 1 (B__keys $? _ = _) => unfold A__keys, B__keys, KEY1, KEY2, KEY__A, KEY__B, KID1, KID2.
+  Hint Extern 1 (PERMS__a $? _ = _) => unfold PERMS__a.
+  Hint Extern 1 (PERMS__b $? _ = _) => unfold PERMS__b.
+  Hint Extern 1 (add _ _ _ $? _ = Some _) => rewrite lookup_add_ne by discriminate.
+  Hint Extern 1 (add _ _ _ = _) => maps_equal; try discriminate.
+  Hint Extern 1 (_ \in _) => sets.
+
+End SimulationAutomation.
+
+Import SimulationAutomation.
+
+Section FeebleSimulates.
+
+  Lemma rpingbase_silent_simulates :
+    forall U__r U__i,
+      RPingPongBase U__r U__i
+      -> forall U__r',
+        rstepSilent U__r U__r'
+        -> exists U__i',
+          istepSilent ^* U__i U__i'
+          /\ RPingPongBase U__r' U__i'.
+  Proof.
+    intros.
+    invert H.
+
+    - churn;
+        (eexists; constructor; swap 1 2; [eapply Start |]; eauto 8).
+
+    - churn;
+        (eexists; constructor; swap 1 2; [eapply Sent1 |]; eauto 8).
+
+    - churn;
+        (eexists; constructor; swap 1 2; [eapply Recd1 |]; eauto 8).
+
+    - churn;
+        (eexists; constructor; swap 1 2; [eapply Sent2 |]; eauto 8).
+
+    - churn;
+        (eexists; constructor; swap 1 2; [eapply Recd2 |]; eauto 8).
+
+    - churn.
+
+  Qed.
+
+  Lemma rpingbase_loud_simulates : 
+    forall U__r U__i,
+      RPingPongBase U__r U__i
+      -> forall a1 U__r',
+        RealWorld.lstep_universe U__r (Action a1) U__r'
+        -> exists a2 U__i' U__i'',
+            istepSilent^* U__i U__i'
+            /\ IdealWorld.lstep_universe U__i' (Action a2) U__i''
+            /\ action_matches a1 a2
+            /\ RPingPongBase U__r' U__i''
+            /\ RealWorld.action_adversary_safe U__r.(RealWorld.adversary) a1 = true.
+  Proof.
+    intros.
+    invert H; churn.
+    
+    unfold ideal_univ_start, RealWorld.updateUniverse, RealWorld.multiMapAdd; simpl.
+
+    - do 3 eexists.
+      propositional; swap 1 4; swap 2 4; swap 3 4;
+        [simplify | | | ]; eauto; eauto 12.
+      admit.
+
+    - do 3 eexists.
+      propositional; swap 1 4; swap 2 4; swap 3 4;
+        [simplify | | | | ]; eauto; eauto 12.
+      admit.
+
+    - do 3 eexists.
+      propositional; swap 1 4; swap 2 4; swap 3 4;
+        [simplify | | | | ]; eauto; eauto 12.
+      admit.
+
+    - do 3 eexists.
+      propositional; swap 1 4; swap 2 4; swap 3 4;
+        [simplify | | | | ]; eauto; eauto 12.
+      admit.
+
+    - do 3 eexists.
+      propositional; swap 1 4; swap 2 4; swap 3 4;
+        [simplify | | | | ]; eauto; eauto 12.
+      admit.
+
+    - do 3 eexists.
+      propositional; swap 1 4; swap 2 4; swap 3 4;
+        [simplify | | | | ]; eauto; eauto 12.
+      admit.
+
+  Admitted.
+
+  Theorem base_pingpong_refines_ideal_pingpong :
+    real_univ_start $0 [] <| ideal_univ_start.
+  Proof.
+    exists RPingPongBase.
+    firstorder; eauto using rpingbase_silent_simulates, rpingbase_loud_simulates.
+  Qed.
+
+End FeebleSimulates. 
+
+Section SingleAdversarySimulates.
+
+  (* If we have a simulation proof, we know that:
+   *   1) No receives could have accepted spoofable messages
+   *   2) Sends we either of un-spoofable, or were 'public' and are safely ignored
+   *
+   * This should mean we can write some lemmas that say we can:
+   *   safely ignore all adversary messages (wipe them from the universe) -- Adam's suggestion, I am not exactly sure how...
+   *   or, prove an appended simulation relation, but I am not sure how to generically express this
+   *)
+
+  Definition add_adversary {A} (U__r : RealWorld.universe A) (advcode : RealWorld.user_cmd A) :=
+    RealWorld.addUniverseUsers U__r [(ADV, {| RealWorld.key_heap := $0 ; RealWorld.protocol := advcode |})].
+
+  Definition strip_adversary {A} (U__r : RealWorld.universe A) : RealWorld.universe A :=
+    {|
+      RealWorld.users            := removelast U__r.(RealWorld.users)
+    ; RealWorld.users_msg_buffer := U__r.(RealWorld.users_msg_buffer)
+    ; RealWorld.all_keys         := U__r.(RealWorld.all_keys)
+    ; RealWorld.all_ciphers      := U__r.(RealWorld.all_ciphers)
+    ; RealWorld.adversary        := U__r.(RealWorld.adversary)
+    |}.
+
+
+  Lemma step_clean_or_adversary :
+    forall {A} (U__r U__ra U__ra' : RealWorld.universe A) advcode lbl u_id u,
+      In (u_id,u) U__r.(RealWorld.users)
+      -> u_id <> ADV
+      -> U__ra = add_adversary U__r advcode
+      -> RealWorld.lstep_universe U__ra lbl U__ra'
+      -> forall stepUdata uks advk cs ks qmsgs (cmd' : RealWorld.user_cmd A),
+          (* Legit step *)
+          ( forall stepUid,
+              In (stepUid,stepUdata) U__r.(RealWorld.users)
+            /\ RealWorld.lstep_user
+                stepUid lbl
+                (RealWorld.universe_data_step U__r stepUdata)
+                (advk, cs, ks, qmsgs, uks, cmd')
+
+          ) \/
+          (* Adversary step *)
+          ( In (ADV,stepUdata) U__ra.(RealWorld.users)
+          /\ RealWorld.lstep_user
+              ADV lbl
+              (RealWorld.universe_data_step U__ra stepUdata)
+              (advk, cs, ks, qmsgs, uks, cmd')
+
+          )
+  .
+  Proof.
+  Admitted.
+
+  Lemma simulates_implies_noninterference:
+    forall {A} (U__r U__ra : RealWorld.universe A) (U__i : IdealWorld.universe A),
+      U__r <| U__i
+      -> forall U__ra' u_id advcode a udata,
+        U__ra = add_adversary U__r advcode
+        -> RealWorld.lstep_universe U__ra (Action a) U__ra'
+        -> RealWorld.lstep_user u_id (Action a) (RealWorld.universe_data_step U__ra udata) (RealWorld.universe_data_step U__ra' udata) 
+        -> In (u_id,udata) U__ra.(RealWorld.users)
+        -> u_id <> ADV.
+  Proof.
+  Admitted.
+
+
+  (* Maybe this isn't provable.  One big question I have is whether we can actually
+   * make the connection for some arbitrary relation.  The biggest problem (maybe)
+   * being that adversaries will certainly affect the book keeping fields of the
+   * simulation relation like: all_keys, all_ciphers, users_message_buffer.
+   * There is no guarantee that the R in the original simulation relation doesn't say
+   * something relevant about those fields.
+   *)
+  Theorem simulates_implies_sim_with_adv :
+    forall {A} (U__r U__ra : RealWorld.universe A) (U__i : IdealWorld.universe A),
+      U__r <| U__i
+      -> forall advcode,
+        U__ra = add_adversary U__r advcode
+        -> U__ra <| U__i.
+  Proof.
+
+  Admitted.
+
+
+
+  (* Can't really write this as is.  Perhaps derive some
+   * kind of traces predicate like in MessagesAndRefinement?  Does that
+   * get to the final theorem we want to prove?
+   *)
+  (* Definition final_answers_agree {A} (U__r : RealWorld.universe A) (U__i : IdealWorld.universe A) : *)
+  (*   forall U__r' U__i', *)
+  (*     RealWorld.lstep_universe^* U__r lbl U__r' *)
+  (*     -> IdealWorld.lstep_universe^* U__i lbl' U__i' *)
+  (*     ->  *)
+
+
+
+
+
+
+
+
+
+  Definition still_simulates_with_adversary (U__i : IdealWorld.universe bool)  (U__r : RealWorld.universe bool) :=
+    U__r <| U__i
+    -> forall U__r' advcode,
+      U__r' = RealWorld.addUniverseUsers U__r [(ADV, {| RealWorld.key_heap := $0 ; RealWorld.protocol := advcode |})]
+      -> U__r' <| U__i.
+
+
+
+    (* Idea:  We have a relation: R : Ureal -> Uideal and need R' : U'real -> Uideal  where U'real is augmented
+     *        with the adversary.  One approach may be to find R'' : U'real -> Ureal and then compose the relations.
+     *        Hrm.  Relations don't really compose...
+     *  What components could go into this R''?
+     *    1. rstepSilent^* -- could provide some support for dropping messages sent by the adversary
+     *    2. some U'real -> Ureal which just peels off the adversary
+     * 
+     * I think the biggest remaining challenge is handling Sends from the adversary.  Should these be 'loud?'
+     *
+     *)
+
+(* How do we augment the simulation relation from above to include an arbitrary adversary? *)
+
+End SingleAdversarySimulates.
