KeyManagement/MessageEq.v
@@ -1,0 +1,10 @@
+Require Import Common.
+Require RealWorld.
+Require IdealWorld.
+
+Import RealWorld.RealWorldNotations.
+Import IdealWorld.IdealNotations.
+
+Inductive message_eq : forall A,  (RealWorld.message A) -> (IdealWorld.message A) -> Prop :=
+| PlaintextMessage : forall content,
+    message_eq (RealWorld.Plaintext content) (IdealWorld.Content content).
